@@ -84,6 +84,7 @@ import Xv6.PipeInv
 import Xv6.PipeRw
 import Xv6.FileDefs
 import Xv6.FileInv
+import Xv6.FtableLock
 import Xv6.SpecKfree
 import Xv6.SpecKalloc
 import Xv6.SpecFreerange
@@ -222,6 +223,7 @@ import Xv6.SpecPipeclose
 import Xv6.SpecPipewrite
 import Xv6.SpecPiperead
 import Xv6.SpecFilealloc
+import Xv6.SpecFiledup
 import Xv6.SpecKfork
 import Xv6.SpecUserinit
 import Xv6.SpecEither
@@ -263,6 +265,10 @@ import Xv6.LinkPipewrite
 import Xv6.ProofPiperead
 import Xv6.LinkPiperead
 import Xv6.ProofFilealloc
+import Xv6.WordFrac
+import Xv6.FileFrac
+import Xv6.ProofFiledup
 import Xv6.LinkFilealloc
+import Xv6.LinkFiledup
 import Xv6.ProofKfork
 import Xv6.LinkKfork
